A few Ideas on PCF-extraction

theories/GenExtract/GenExtractPCF.v
@@ -1,4 +1,4 @@
-From Undecidability Require Import L.Tactics.ComputableTime GenExtract.utlc_syntax.
+From Undecidability Require Import L.Tactics.ComputableTime GenExtract_syntax.
 From Undecidability Require Import LNat.
 
 Import fintype.
@@ -6,6 +6,17 @@ Set Universe Polymorphism.
 Local Unset Implicit Arguments.
 (*Set Printing Universes. *)
 
+(* Hints from Yannick: *)
+(* See "Oef", Denotational semantics . *)
+(* See Buss Splitters, Denotational semantics for smart contracts **)
+(* Pieres thesis: "egal wie rekursion geht, immer beweisbar extrahierbar"*)
+(* Yannick Forster, [03.09.20 16:18]
+Es könnte auch hilfreich sein nochmal auf eine (zum Beispiel kategorientheoretische) denotational semantics vom STLC zu gucken, oder sogar auf eine von PCF
+
+Yannick Forster, [03.09.20 16:18]
+Denke deine Relation ist exakt eine denotationelle Semantik -Relation, geinlined mit dem typing judgement
+
+*)
 Module Env.
 
   
@@ -22,16 +33,31 @@ Module Env.
     fin_to_nat f < n.
   Proof. induction n in f|-*;cbn in *. easy. destruct f. specialize (IHn f).  all:nia. Qed.
 
-  Fixpoint nat_to_fin n k : k < n -> fin n :=
+  Fixpoint nat_to_fin {n k} : k < n -> fin n :=
     match n with
       0 => fun H => @False_rect _ (Nat.nle_succ_0 _ H)
     | S n => match k with
               0 => fun _ => None
-            | S k => fun H => Some (nat_to_fin n k (Peano.le_S_n _ _ H))
+            | S k => fun H => Some (@nat_to_fin n k (Peano.le_S_n _ _ H))
             end
     end.
 
-  (*
+  
+  Lemma nat_to_fin_unique {n i} (H1 H2 : i < n) :
+    nat_to_fin H1 = nat_to_fin H2.
+  Proof.
+    unfold lt in *. replace H2 with H1. easy. apply le_unique.
+  Qed.
+
+  
+  Lemma fin_to_nat_inv n k (H : k < n):
+    fin_to_nat (nat_to_fin H) = k.
+  Proof. induction n in k,H|-*;cbn. easy. destruct k. easy. now rewrite IHn. Qed.
+
+  Definition lift_closed {n} : fin 0 -> fin n := False_rect _.
+
+
+(*
   Fixpoint vec (X:Type) n : Type :=
     match n with
       0 => unit
@@ -67,6 +93,73 @@ Module Env.
 End Env.
 Import Env.
 
+
+Section scopedSyntax.
+  
+  Fixpoint utlc_to_term {n} (s:utlc n) : term :=
+    match s with
+      var_utlc x => var (fin_to_nat x)
+    | appUtlc s t=> L.app (utlc_to_term s) (utlc_to_term t)
+    | lamUtlc s => L.lam (utlc_to_term s)
+    end.
+  
+  Lemma utlc_to_term_bound n (s: utlc n) :
+    bound n (utlc_to_term s).
+  Proof. induction s;cbn. 1:specialize (fin_to_nat_lt f). all:eauto using bound. Qed.
+
+  Definition term_to_utlc' : forall {n} s, bound n s -> utlc n.
+  Proof.
+    refine ((fix term_to_utlc n s :=
+               match s with
+                 L.var x => fun H => var_utlc (@nat_to_fin n x _)
+               | L.app s t => fun H => appUtlc (term_to_utlc n s _)  (term_to_utlc n t _)
+               | L.lam s => fun H => lamUtlc (term_to_utlc (S n) s _)
+               end)
+              ). all:abstract now inv H.
+  Defined.
+
+  Definition term_to_utlc s (H:closed s) : utlc 0 := term_to_utlc' s (closed_dcl_x 0 H).
+  
+  Definition r__utlc : utlc 0:= term_to_utlc r ltac:(unfold r;Lproc). 
+
+  Definition rho__utlc {n} (s : utlc n) : utlc n :=
+    lamUtlc (appUtlc (appUtlc ((appUtlc r__utlc r__utlc)⟨ lift_closed ⟩)
+                              (s ⟨ shift ⟩ ) )
+                     (var_utlc (nutlc := S n) None)).
+
+  Lemma rho_utlc_to_term {n} (s : utlc n):
+    utlc_to_term (rho__utlc s) = rho (utlc_to_term s ⟨ shift ⟩ ).
+  Proof. reflexivity. Qed.
+
+  Lemma rho_utlc_subst n m (s : utlc n) (σ: fin n -> utlc m):
+    ltac:(let H := eval cbv [subst1 Subst_utlc] in (((rho__utlc s) [σ]) = rho__utlc (s[ σ ])) in exact H).
+  Proof. unfold rho__utlc;asimpl. reflexivity. Qed. 
+  
+  Lemma utlc_to_term_inv' n s (H: bound n s):
+    utlc_to_term (@term_to_utlc' n s H) = s.
+  Proof.
+    induction s in n,H |-*. all:cbn.
+    -now rewrite fin_to_nat_inv. 
+    -now rewrite IHs1, IHs2.
+    -now rewrite IHs.
+  Qed.
+
+
+  Lemma utlc_to_term_inv s H n τ:
+    ltac:(let H := eval cbv [subst1 Subst_utlc] in (utlc_to_term (n:=n) ((term_to_utlc s H) [τ]) = s) in exact H).
+  Admitted.
+
+  Lemma term_to_utlc_PI s H H' :
+    term_to_utlc s H = term_to_utlc s H'.
+  Admitted.
+
+  
+  Lemma proc_shift n (s : utlc n) :
+    closed (utlc_to_term s) ->  utlc_to_term (s ⟨↑⟩) = utlc_to_term s.
+  Admitted.
+
+End scopedSyntax.
+
 (*
 Polymorphic Inductive TT : Type -> Type :=
   TyNat : TT nat
@@ -84,6 +177,21 @@ Hint Mode TT + : typeclass_instances. (* treat argument as input and force evar-
 
 (** Extract only very basic functions, which are more or less PCF with "coq-guarded" recursion *)
 
+
+Definition  PCFtoL : forall {n} (s: pcf n), utlc n.
+  refine ((fix PCFtoL n s : utlc n:=
+  match s with
+  | var_pcf x => var_utlc x
+  | constPcf c => (term_to_utlc (enc c) _) ⟨lift_closed⟩
+  | appPcf s t => appUtlc (PCFtoL _ s) (PCFtoL _ t)
+  | lamPcf s => lamUtlc (PCFtoL (S n) s)
+  | fixPcf s => rho__utlc (lamUtlc ((PCFtoL _ s)⟨shift ⟩))
+  | caseNatPcf s t u => appUtlc (appUtlc (PCFtoL _ s) (PCFtoL _ t)) (PCFtoL _ u)
+  | succPcf => (term_to_utlc (ext S) _) ⟨lift_closed⟩
+  end)).
+  all:abstract Lproc.
+Defined. 
+
 Record anyTT := {aTy : Type ; aTT :> TT aTy}.
 
 Coercion Build_anyTT : TT >-> anyTT.
@@ -92,52 +200,59 @@ Existing Instance Build_anyTT.
 
 Notation vec := (fun X n => (fin n -> X)).
 
-
-
 Definition hvec {X} (F: X -> Type) {n} : (fin n -> X) -> Type :=
   fun sigma => forall i, F (sigma i).
+
+Definition hvec_cons {X:Type} (F:X -> Type)
+           (x : X) (v:F x)  {n} xs (vs : hvec (n:=n) F xs) : hvec (n:=S n) F (x.:xs)
+  := fun i => match i with None => v | Some i => vs i end.
+
+Local Notation "h '.::' t" := (@hvec_cons _ _ _ h _ _ t) (at level 55, right associativity).
+
 
 Notation typeContext := (vec anyTT).
 Notation valueContext := (hvec aTy).
 
-Local Unset Implicit Arguments.
 
+
+Local Unset Implicit Arguments.
 
 Notation TyNat := (@TyB _ registered_nat_enc).
 
-Inductive isPCF : forall n (Γ : typeContext n) (A: anyTT), (valueContext Γ -> A.(aTy)) -> Type :=
+Inductive isPCF : forall n (Γ : typeContext n) (A: anyTT), (valueContext Γ -> A.(aTy)) -> (pcf n) -> Type :=
   isPCF_Const n Γ (c:nat) :
-    isPCF n Γ TyNat (fun _ => c)
-| isPCF_Rel n Γ x : isPCF n Γ (Γ x ) (fun sigma => sigma x)
-| isPCF_App n Γ (A B : anyTT)
+    isPCF n Γ TyNat (fun _ => c) (constPcf c)
+| isPCF_Rel n Γ x : isPCF n Γ (Γ x ) (fun sigma => sigma x) (var_pcf x)
+| isPCF_App n Γ s t(A B : anyTT)
             (f:valueContext Γ -> A.(aTy) -> B.(aTy)) (arg: valueContext Γ -> A.(aTy)):
-    isPCF n Γ (TyArr A B) f
-    -> isPCF n Γ A arg
-    -> isPCF n Γ B (fun ctx => (f ctx) (arg ctx))
-| isPCF_Lambda n (Γ : typeContext n) A B (f:valueContext Γ -> _):
-    isPCF (S n) (A.:Γ) B (fun ctx => f (fun x => ctx (Some x)) (ctx None))
-    -> @isPCF n Γ (TyArr A B) f
-             
-| isPCF_Case_nat n Γ A x (f__O : valueContext Γ -> A.(aTy)) (f__S: valueContext Γ -> nat -> A.(aTy)):
-    isPCF n Γ TyNat x
-    -> isPCF n Γ A f__O 
-    -> isPCF n Γ (TyArr TyNat A) f__S (* "inlining" means that we can reuse the Lambda-part of proofs *)
-    -> isPCF n Γ A (fun ctx => match x ctx with 0 => f__O ctx | S n => f__S ctx n end)
+    isPCF n Γ (TyArr A B) f s
+    -> isPCF n Γ A arg t
+    -> isPCF n Γ B (fun ctx => (f ctx) (arg ctx)) (appPcf s t)
+| isPCF_Lambda n (Γ : typeContext n) s A B (f:valueContext Γ -> _):
+    isPCF (S n) (A.:Γ) B (fun ctx => f (fun x => ctx (Some x)) (ctx None)) s
+    -> @isPCF n Γ (TyArr A B) f (lamPcf s)
+| isPCF_Case_nat n Γ s__x s__O s__S A x (f__O : valueContext Γ -> A.(aTy)) (f__S: valueContext Γ -> nat -> A.(aTy)):
+    isPCF n Γ TyNat x s__x
+    -> isPCF n Γ A f__O s__O
+    -> isPCF n Γ (TyArr TyNat A) f__S s__S (* "inlining" means that we can reuse the Lambda-part of proofs *)
+    -> isPCF n Γ A (fun ctx => match x ctx with 0 => f__O ctx | S n => f__S ctx n end) (caseNatPcf s__x s__O s__S)
              
 | isPCF_Succ n Γ:
-    @isPCF n Γ (TyArr _ _) (fun _ => S)
-| isPCF_Fix_unaryNat n Γ (A:anyTT) f (F : valueContext Γ -> nat -> A.(aTy))
-                     (H__Fix : forall (ctx : valueContext Γ) (x:nat), F ctx x = f ctx (F ctx) x) :
-    isPCF n Γ (TyArr (TyArr TyNat A) (TyArr TyNat A)) f
-    -> isPCF n Γ {|aTT := TyArr TyNat A|} (fun ctx x => F ctx x).
+    @isPCF n Γ (TyArr _ _) (fun _ => S) (succPcf)
+| isPCF_Fix_unaryNat n Γ s (A:anyTT)
+                     (f : valueContext Γ -> (nat -> aTy A) -> nat -> aTy A)
+                     (F : valueContext Γ -> nat -> A.(aTy))
+                     (eq__fun : forall (ctx : valueContext Γ) (x:nat), F ctx x = f ctx (F ctx) x)
+                     (*
+                     (H__ind : forall (P : (nat -> aTy A) -> Type),
+                         (forall ctx f', P f' -> P (f ctx f'))
+                         -> forall ctx, P (F ctx))*):
+    (*TODO: how exactly does recursion work in general: how is the functional recurrsor connected to functional recursion principle? *)
 
-Arguments isPCF_Const {n Γ} c.
-Arguments isPCF_Rel {n Γ} _.
-Arguments isPCF_App {n Γ A B f arg}.
-Arguments isPCF_Lambda {n Γ A B f}.
-Arguments isPCF_Case_nat {n Γ A x f__O f__S}.
-Arguments isPCF_Succ {n Γ}.
-Arguments isPCF_Fix_unaryNat {n Γ A f F _} _.
+    (* Note: I expect that P must be extensional in the first argument. *)
+    isPCF n Γ (TyArr (TyArr TyNat A) (TyArr TyNat A)) f s
+    -> isPCF n Γ {|aTT := TyArr TyNat A|} (fun ctx x => F ctx x) (fixPcf s).
+
 
 Arguments isPCF {_} _ _ _.
 
@@ -145,15 +260,23 @@ Arguments isPCF {_} _ _ _.
 
 (*Lemma isPCF_mono : isPCF n Γ tt f *)
 
-Lemma isPCF_plus n (Γ: typeContext n): isPCF Γ (TyArr _ (TyArr _ _)) (fun _ => plus).
+Lemma isPCF_plus n (Γ: typeContext n): { s & isPCF Γ (TyArr _ (TyArr _ _)) (fun _ => plus) s}.
 Proof.
-  unfold Init.Nat.add.
+  unfold Init.Nat.add. eexists.
   apply @isPCF_Fix_unaryNat with (A := {| aTT := (TyArr TyNat TyNat) |} )
                                  (f:= fun ctx=> fun F n m => match n  with
                                                    | 0 => m
                                                    | S p => S (F p m)
                                                    end).
   now intros arg [].
+  (*
+  {fold plus. intros P IH ctx. specialize (IH ctx). cbn in *. change (fun x : nat => Init.Nat.add x) with plus in *.
+   specialize IH with (f':=plus) as IH'.
+   fix REC 1. intros [|n']. all:cbn.
+   -clear REC. specialize (IH 0). cbn in IH. apply IH. refine (IH _ _). cbn in IH. eapply IH. eassumption. specialize (REC 0). cbn in REC. exact REC. Guarded. destruct x.
+   -refine (f' := )
+   induction x. eapply IH. 
+   change (fun x y : nat => Init.Nat.add x y) with plus in *.  cbn in P. *)
   eapply @isPCF_Lambda with (A := (TyNat ~> TyNat ~> TyNat)) (B := (TyNat ~> TyNat ~> TyNat)).
   eapply @isPCF_Lambda with (A := TyNat) (B := (TyNat ~> TyNat)).
   eapply @isPCF_Lambda with (A := TyNat) (B := TyNat).
@@ -169,90 +292,14 @@ Proof.
    now eapply @isPCF_Rel with (x:=None).
 Defined.
 
-Import utlc_syntax.
-Section scopedSyntax.
-  Fixpoint tm_to_term {n} (s:tm n) : term :=
-    match s with
-      var_tm x => var (fin_to_nat x)
-    | app s t=> L.app (tm_to_term s) (tm_to_term t)
-    | lam s => L.lam (tm_to_term s)
-    end.
-  
-  Lemma tm_to_term_bound n (s: tm n) :
-    bound n (tm_to_term s).
-  Proof. induction s;cbn. 1:specialize (fin_to_nat_lt f). all:eauto using bound. Qed.
-
-  Definition term_to_tm : forall s n, bound n s -> tm n.
-  Proof.
-    refine (fix term_to_tm s n H =>
-            match s with
-              L.var x => var_tm 
-  
-
-
-
-Fixpoint PCFtoL {n} {Γ : typeContext n} {A:anyTT} {f:valueContext Γ -> A.(aTy)} (H : isPCF Γ A f): vec nat n -> tm n :=
-  match H with
-  | @isPCF_Const n Γ c => fun ren => enc c
-  | @isPCF_Rel n Γ x =>  fun ren => var (ren x)
-  | @isPCF_App n Γ A B f arg H__f H__arg =>  fun ren => app (PCFtoL H__f ren) (PCFtoL H__arg ren)
-  | @isPCF_Lambda n Γ A B f H__f =>  fun ren => lam (PCFtoL H__f (shift ren))
-
-  (* TODO: lambda-lift for "lazy" evaluation?*)
-  | @isPCF_Case_nat n Γ A x f__O f__S H__x H__O H__S =>  fun ren => app (app (PCFtoL H__x ren) (PCFtoL H__O ren)) (PCFtoL H__S ren)
-                                                  
-  | @isPCF_Succ n Γ =>  fun ren => ext S
-  | @isPCF_Fix_unaryNat n Γ A f F H__Fix H__F =>  fun ren => rho ((PCFtoL H__F (Some >> ren)))
-  end.
-
-Fixpoint vec_to_list {n X} : vec X n -> list X :=
-  match n with
-    0 => fun _ => nil
-  | S n => fun xs => fst xs :: vec_to_list (snd xs)
-  end.
-
-Lemma vec_to_list_In {X n} (x:X) (v:vec X n):
-  In x (vec_to_list v) -> exists i, nth__V i v = x.
-Proof.
-  induction n;cbn in *. easy. intros [ <- | ]. now eexists None.
-  edestruct IHn as [i ?]. eauto. now eexists (Some i).
-Qed.
-
-Lemma vec_to_list_length {n X} (xs : vec X n):
-  length (vec_to_list xs) = n.
-Proof. induction n in xs |-*;cbn. easy. now rewrite IHn. Qed.
-
-Fixpoint nat_to_fin {n i} : i < n -> fin n.
-  refine (match n with
-            0 => fun H => False_rect _ _
-          | S n => match i as i return i < (S n) -> fin (S n) with
-                    0 => fun _ => None
-                  | S i => fun H => Some (@nat_to_fin n i _)
-                  end
-          end).
-  all:abstract nia.
-Defined.
-
-Lemma nat_to_fin_unique {n i} (H1 H2 : i < n) :
-  nat_to_fin H1 = nat_to_fin H2.
-Proof.
-  unfold lt in *. replace H2 with H1. easy. apply le_unique.
-Qed.
-
-
-Lemma vec_to_list_nth n X (vs:vec X n) i (H : i < n) d:
-  nth i (vec_to_list vs) d = nth__V (nat_to_fin H) vs.
-Proof.
-  induction n in vs,i,H |-*. nia. destruct vs. cbn.
-  destruct i. easy. erewrite IHn. reflexivity.
-Qed.
-
+(*
 Lemma extensionalMatch_nat {X} (T : X -> Type) n H__O H__S:
   T (match n with 0 => H__O | S n => H__S n end) = match n with 0 => T H__O | S n => T (H__S n) end.
 Proof.
   now destruct n.
 Defined.
 
+ *)
 
 Lemma dualMatch_nat X Y (T : X -> Y -> Type) n H1__O H1__S H2__O H2__S:
   T (match n with 0 => H1__O | S n => H1__S n end) (match n with 0 => H2__O | S n => H2__S n end) = match n with 0 => T H1__O H2__O | S n => T (H1__S n) (H2__S n) end.
@@ -260,13 +307,15 @@ Proof.
   now destruct n.
 Defined.
 
-
+(*
 Lemma nat_case {X} (T : X -> Type) H__O H__S:
   T H__O -> (forall n, T (H__S n)) -> forall n, T (match n with 0 => H__O | S n => H__S n end).
 Proof.
   now intros ? ? [].
 Defined.
+ *)
 
+(*
 Lemma substList_rho s k A:
   LClos.substList (rho s) k A = rho (LClos.substList s (S k) A).
 Proof.
@@ -290,7 +339,9 @@ Proof. induction n in xs|-*;cbn. easy. rewrite IHn.  reflexivity. Qed.
 Lemma hvec_impl {X} {P Q} {n} (xs : vec X n):
   (forall x, P x -> Q x) -> hvec P xs -> hvec Q xs.
 Proof. induction n in xs|-*;cbn. easy. intros ? [];split. all:eauto. Qed.
+ *)
 
+(*
 Lemma bound_PCFtoL {n} {Γ : typeContext n} {A:anyTT} {f:valueContext Γ -> A.(aTy)}
       (H : isPCF Γ A f) (ren : vec nat n) k:
   hvec (fun x => x < k) ren
@@ -316,8 +367,9 @@ Proof.
   -rewrite IHisPCF. easy. unfold up;split;cbn. easy. rewrite hvec_map. eapply hvec_impl with (2:=Hneq). nia.
   -rewrite subst_rho, IHisPCF. easy. rewrite hvec_map. eapply hvec_impl with (2:=Hneq). nia.
 Qed.
+*)
 
-
+(*
 Lemma subst_substList_swap s k A x u:
   bound k u
   -> x < k
@@ -374,44 +426,46 @@ Proof.
   -cbn;now  f_equal.
   -cbn. unfold up. cneauto. 
 *)
-
-Lemma isPCF_L_computable {n} {Γ : typeContext n} {A:anyTT} {f:valueContext Γ -> A.(aTy)}
-      (H : isPCF Γ A f) (vs : valueContext Γ) k (env__L : vec term k) (ren : vec nat n) 
-      (proc__env  : hvec proc env__L) (bound__ren : hvec (fun x => x < k) ren):
-  (forall i, computes (nth__V i Γ).(aTT) (nth__HV i vs) (nth__V (nat_to_fin (nth__HV i bound__ren)) env__L))
-  -> {v & (LClos.substList (PCFtoL H ren) 0 (vec_to_list env__L) >* v) * computes A.(aTT) (f vs) v}%type.
+*)
+Set Nested Proofs Allowed.
+Lemma isPCF_L_computable {n} {Γ : typeContext n} {A:anyTT} {f:valueContext Γ -> A.(aTy)} {s__f}
+      (H : isPCF Γ A f s__f) (vs : valueContext Γ) k (env__L : vec (utlc 0) k) (τ : vec (fin k) n):
+  ltac:(let H := eval cbv [subst1 Subst_utlc] in 
+        ((forall i, computes (Γ i).(aTT) (vs i) (utlc_to_term (env__L (τ i))))
+        -> {v & (utlc_to_term ((PCFtoL s__f) [ τ >> env__L]) >* v)  * computes A.(aTT) (f vs) v}%type) in exact H).
 Proof.
-  revert k env__L proc__env bound__ren.
-  induction H;intros k env__L proc__env bound__ren H__env.
-  1:{(* Const*) do 2 esplit. cbn. rewrite LClos.substList_closed. 1,3:reflexivity. Lproc. }
-  1:{(*Rel*) cbn. rewrite Nat.sub_0_r. do 2 esplit. reflexivity.
-     erewrite vec_to_list_nth. apply H__env. 
+  revert k env__L τ vs.
+  induction H;intros k env__L τ vs H__env.
+  1:{cbn. (* Const*) eexists.
+     assert (H:= utlc_to_term_inv ). asimpl. rewrite H. split. all:reflexivity. }
+  1:{(*Rel*) cbn. do 2 esplit. reflexivity. apply H__env. 
   }
-  1:{(*App*) cbn. edestruct IHisPCF2  with (1:=proc__env) (bound__ren:=bound__ren) (2:=H__env) as (v2&R2&IH2). 
-      cbn in IHisPCF1. edestruct IHisPCF1 with (2:=H__env) as (v&R&Hproc&v'&R'&IH1) . 1,2:eassumption. 
+  1:{(*App*) cbn. edestruct IHisPCF2  with (1:=H__env) as (v2&R2&IH2). 
+      cbn in IHisPCF1. edestruct IHisPCF1 with (1:=H__env) as (v&R&Hproc&v'&R'&IH1) . 1:eassumption. 
       eexists;split. 2:easy. rewrite R,R2. easy.
   }
   1:{ (*Lambda *) cbn.
       eexists. split. reflexivity. split. split. 2:easy.
-      { (*PCFtoL is closed *) apply closed_dcl. constructor. apply LClos.substList_is_bound.
-        1:now apply validEnv'_vec_to_list. rewrite vec_to_list_length. now  eapply bound_PCFtoL, bound_up. }
-      intros.
-      unshelve edestruct IHisPCF with (k:= S k) (vs := (a,vs)) (env__L := (t_a,env__L)) (ren := (up ren)) as (v&R&IH).
-      {now apply  bound_up. }
-      {split;cbn. all:eauto using computesProc. }
-      {intros []. 2:assumption. cbn.
-       set (l:=nth__HV f0 (snd (bound_up _ k ren bound__ren))). cbn in l. fold l. generalize l. clear l.
-       rewrite nthV_mapV. intros ?. cbn. erewrite nat_to_fin_unique. apply H__env.
-      }
+      { (*PCFtoL is closed *) apply closed_dcl. constructor. apply utlc_to_term_bound. }
+      intros a t__a Ha.
+      unshelve edestruct IHisPCF with (k:= S k) (vs := a.::vs) (env__L := term_to_utlc t__a (proc_closed (computesProc Ha)) .:env__L) (τ:=up_ren τ) as (v&R&IH).
+      { intros []. all:cbn - [computes]. now eapply H__env. now setoid_rewrite utlc_to_term_inv'. }
       cbn in IH.
       eexists. split. 
       rewrite step_Lproc. 2:now eapply computesProc. 2:exact IH.
-      rewrite LClos.subst_substList. eassumption. now eapply validEnv'_vec_to_list.
+      
+      Lemma subst_utlc_to_term s (t : utlc 0):
+        ltac:(let H := eval cbv [subst1 Subst_utlc] in (
+              subst (utlc_to_term s) 0 (utlc_to_term t) = utlc_to_term s [t.:(id >> var_utlc)]) in exact H).
+      Admitted. 
+      unshelve erewrite <- utlc_to_term_inv' with (n:=0) (s:=t__a). (clear - Ha;eapply computesProc in Ha; Lproc'). 
+      rewrite subst_utlc_to_term.
+      erewrite term_to_utlc_PI in R. asimpl in *. exact R.
   }
   1:{ (* Case_nat *) cbn.
-      specialize IHisPCF1 with (vs:=vs) (ren:=ren) (env__L := env__L) (1:=proc__env) (bound__ren:=bound__ren) (2:=H__env).
-      specialize IHisPCF2 with (vs:=vs) (ren:=ren) (env__L := env__L) (1:=proc__env) (bound__ren:=bound__ren) (2:=H__env).
-      specialize IHisPCF3 with (vs:=vs) (ren:=ren) (env__L := env__L) (1:=proc__env) (bound__ren:=bound__ren) (2:=H__env).
+      specialize IHisPCF1 with (vs:=vs) (τ:=τ) (env__L := env__L) (1:=H__env).
+      specialize IHisPCF2 with (vs:=vs) (τ:=τ) (env__L := env__L) (1:=H__env).
+      specialize IHisPCF3 with (vs:=vs) (τ:=τ) (env__L := env__L) (1:=H__env).
 
       edestruct IHisPCF1 as (_ &R__x &[= -> ]).
       edestruct IHisPCF2 as (v__O &R__O &IH__O).
@@ -435,62 +489,41 @@ Proof.
       set (IH := (snd (projT2 IH__v))). subst IH__v.
       exact IH.
   }
-  1:{(* Succ *) eexists;split. reflexivity. cbn - [computes]. rewrite LClos.substList_closed. 2:now Lproc. apply extCorrect. }
-  1:{(* Fix_unaryNat *) cbn - [rho].
-     rewrite substList_rho.
-     set (REC' := LClos.substList _ _ _).  set (REC := rho REC').
-     assert (cls__REC' : proc REC).
+  1:{(* Succ *) eexists;split. reflexivity. cbn - [computes]. asimpl.
+     setoid_rewrite utlc_to_term_inv. apply extCorrect. }
+  1:{(* Fix_unaryNat *) cbn - [rho__utlc]. auto_unfold in *. 
+     rewrite rho_utlc_subst.
+     asimpl.
+     set (σ:=τ >> (env__L >> ⟨↑⟩)).  auto_unfold in *.  fold σ. 
+     set (REC' := lamUtlc (PCFtoL s)[σ]). auto_unfold in *. fold REC'.
+     assert (cls__REC' : proc (utlc_to_term REC')).
      {
-       split. 2:unfold REC;cbn;now eexists.
-       unfold REC, REC'. apply closed_dcl. apply rho_dcls, LClos.substList_is_bound. 
-       1:now apply validEnv'_vec_to_list. rewrite vec_to_list_length.
-       eapply bound_PCFtoL. now eapply bound_shift.
+       split. 2:unfold REC';cbn;now eexists.
+       unfold REC'. apply closed_dcl. eapply utlc_to_term_bound.  
      }
-     eexists. split. reflexivity. split. easy. 
+     eexists. split. reflexivity. split.
+     { split. 2:apply rho_lambda. apply closed_dcl, utlc_to_term_bound. }
      
      intros x ? ->.
-     (* TODO: understand how to match 0 in IisPCF with 1 in REC'. I trued k = S k below, but that seeemed srange  *)
-     (*
-     Set Nested Proofs Allowed.
-     Goal forall s t u, app (rho (lam s)) (lam t) >* u.
-     Proof.
-       intros ? ? ?.
-       unfold rho. repeat (econstructor;[now repeat constructor|cbn ] ).
-       assert (H:=eq_refl (rho (lam s))). unfold rho in H at 2. cbv - [rho] in H. rewrite <- H. eqn:H. 
-       fold (rho (lam s)).
-       refine (_ : (app _ (rho (lam s))) >* _).
-       fold subst.
-      *)
-     unshelve specialize IHisPCF with (k:=k) (vs := vs) (env__L := env__L) (ren:= map__V S ren) as (v__f&R__f&proc__f&IH__f).
-     (*1,2,3:easy. *)(*now apply bound_shift.
-     1:now split;cbn.
-     1:{ intros i. erewrite nat_to_fin_unique. apply H__env. eassumption. re cbn. } *)
-     (*
-     fold REC in R__f. rewrite substList_rho.
-     cbn in R__f. rewrite <- LClos.subst_substList in R__f. 2:now apply validEnv'_vec_to_list.
-     rewrite subst_substList_unused_var in R__f. 3:now eapply validEnv'_vec_to_list.
-     2:{ apply PCFtoL_unused_vars. rewrite hvec_map. eapply hvec_impl with (2:=bound__ren). nia. } *)
+     rewrite rho_utlc_to_term,proc_shift. 2:Lproc.
+     specialize IHisPCF with (env__L:=env__L) (τ:=τ) (vs:=vs) (1:=H__env) as (v&R&IH).
+     specialize (eq__fun vs x).
 
      
-     (* TODO: incorperate "recursion" into isPCF_Fix_unaryNat  *)
-     specialize IH__f with (a:= F vs) (t_a := REC).
+     
+     (*      edestruct IH as (v'&?R'&v''&IH'). shelve. 
+
+     hnf in IH'. *)
+     
+     (*explore *)eexists;split.
+     rewrite rho_correct. 2,3:now Lproc. unfold REC' at 1. cbn - [REC'].
+     rewrite step_Lproc at 1. 2:Lproc.
+     rewrite <- proc_shift with (s:=REC') at 1. 2:Lproc. rewrite <- rho_utlc_to_term.
+     rewrite subst_utlc_to_term. unfold σ. asimpl.
+     rewrite R. reflexivity.
+
+     (* TODO: instead of explore, extend isPCF to allow recursion/induction.
+Or think what functional induction/recursion is in general. *)
      admit.
-     
-         hnf in IH__f. 
-         eexists;split. 
-         rewrite PCFtoL_unused_vars in R__f.
-         2:{ apply LClos.substList_is_bound.  }
-         
-
-         eexists. split. rewrite rho_correct. 3:Lproc. 2:admit.
-
-         Lemma substList_
-         rewrite LClos.substList_bound.
-     2:{ eapply bound_PCFtoL. }
-     ).
-     rewrite LClos
-     setoid_rewrite substList_rho. rewrite rho_correct.
-     2:{ }
-     2:  (*PCFtoL is closed *) admit. 2:Lproc. all:admit (*TODO: recursion *). 
   }
-Admitted.
+Admitted. 
